src/two/protocol.v
@@ -35,7 +35,7 @@ Context `{!invGS Σ}.
 *)
 
 Record StorageMixin P B
-    `{Equiv P, PCore P, Op P, Valid P, Inv P}
+    `{Equiv P, PCore P, Op P, Valid P, PInv P}
     {equ: @Equivalence P (≡)}
     `{Equiv B, PCore B, Op B, Valid B, Unit B}
 := {
@@ -44,7 +44,8 @@ Record StorageMixin P B
     
     interp: P -> B;
 
-    interp_proper: Proper ((≡) ==> (≡)) (@inv P _);
+    interp_proper: Proper ((≡) ==> (≡)) interp;
+    interp_val: ∀ p: P , pinv p -> ✓ interp p;
 }. 
 
 Section PropMap.
@@ -60,41 +61,139 @@ Section PropMap.
   
 End PropMap.
 
-Section StorageDefs.
-  Context `{Equiv B, PCore B, Op B, Valid B, Unit B}.
-  Context `{Equiv P, PCore P, Op P, Inv P, Valid P}.
-  Context {equ: Equivalence (≡@{P})}.
-  Context {storage_mixin: StorageMixin P B}.
-
-  Definition storage_protocol_guards (p: P) (b: B) :=
-      ∀ q , inv (p ⋅ q) -> b ≼ interp P B storage_mixin (p ⋅ q).
-  
-End StorageDefs.
-
 Section StorageLogic.
   Context `{Equiv B, PCore B, Op B, Valid B, Unit B}.
-  Context `{Equiv P, PCore P, Op P, Inv P, Valid P}.
+  Context `{Equiv P, PCore P, Op P, PInv P, Valid P}.
   Context {equ: Equivalence (≡@{P})}.
+  Context {equb: Equivalence (≡@{B})}.
   Context {storage_mixin: StorageMixin P B}.
+  
+  Definition storage_protocol_guards (p: P) (b: B) :=
+      ∀ q , pinv (p ⋅ q) -> b ≼ interp P B storage_mixin (p ⋅ q).
   
   Context {Σ: gFunctors}.
   Context `{!inG Σ (authUR (inved_protocolUR (protocol_mixin P B storage_mixin)))}.
   Context `{!invGS Σ}.
   
   Definition maps (γ: gname) (f: B -> iProp Σ) : iProp Σ :=
-      ⌜ wf_prop_map f ⌝ ∗
+      ⌜ wf_prop_map f /\ (∃ p: P , True) ⌝ ∗
       ownI γ (
         ∃ (state: P) ,
           own γ (● (Inved state))
-          ∗ ⌜ inv state ⌝
+          ∗ ⌜ pinv state ⌝
           ∗ (f (interp P B storage_mixin state))
       ). 
   
   Definition p_own (γ: gname) (p: P) : iProp Σ := own γ (◯ (Inved p)).
   
-  Lemma logic_guard (p: P) (b: B)
+  Lemma ownIagree (γ : gname) (X Y : iProp Σ) : ownI γ X ∗ ownI γ Y ⊢ (▷ X ≡ ▷ Y).
+  Admitted.
+  
+  Lemma and_later_r (X Y : iProp Σ)
+      : X ∧ ▷ Y ⊢ ▷ (X ∧ Y). Admitted.
+  
+  (*Lemma logic_guard_conjunct_fact (γ: gname) (p state: P) (f: B -> iProp Σ)
+  : own γ (◯ Inved p)
+        ∧ ▷ (own γ (● Inved state) ∗ ⌜pinv state⌝ ∗ f (interp P B storage_mixin state))
+    ⊢ ⌜ p ≼ state ⌝.
+  Proof.
+    iIntros "x".
+    iDestruct (and_later_r with "x") as "x".
+    iMod "x" as "x".*)
+  
+  Lemma and_timeless (X Y : iProp Σ) (ti: Timeless Y)
+      : ⊢ (X ∧ (▷ Y) -∗ ◇ (X ∧ Y)) % I.
+  Proof.
+    iIntros "r". unfold Timeless in ti.
+    rewrite bi.except_0_and.
+    iSplit. { iDestruct "r" as "[r _]". iModIntro. iFrame. }
+    iDestruct "r" as "[_ r]".  iDestruct (ti with "r") as "r". iFrame.
+  Qed.
+  
+  Lemma and_timeless2 (X Y : iProp Σ) (ti: Timeless Y)
+      : ⊢ (X ∧ (▷ Y) ={∅}=∗ (X ∧ Y)) % I.
+  Proof.
+    iIntros "x".  iMod (and_timeless with "x") as "x". iModIntro. iFrame.
+  Qed.
+  
+  Lemma apply_timeless (X Y Z W V : iProp Σ) (ti: Timeless Z) (ti2: Timeless W)
+      : X ∧ (Y ∗ ▷ (Z ∗ W ∗ V)) -∗ ◇ (X ∧ (Y ∗ Z ∗ W ∗ ▷ (V))).
+      Admitted.
+      
+  Lemma stuff1 (X Y Z W V : iProp Σ)
+      : (X ∧ (Y ∗ Z ∗ W ∗ V)) ⊢ W. Admitted.
+      
+  Lemma stuff2 (γ: gname) (p state: P) (T W: iProp Σ)
+      : own γ (◯ Inved p) ∧ (T ∗ own γ (● Inved state) ∗ W)
+          ⊢ ⌜ p ≼ state ⌝. Admitted.
+  
+  Lemma logic_guard (p: P) (b: B) (γ: gname) (f: B -> iProp Σ)
     (g: storage_protocol_guards p b)
-    : maps γ f ⊢ p_own γ p &&{ {[ γ ]} }&&> f b.
+    : maps γ f ⊢ (p_own γ p &&{ {[ γ ]} }&&> ▷ f b).
+  Proof.
+    unfold guards, guards_with, maps.
+    iIntros "[%wf #inv]".
+    destruct wf as [wf exists_p].
+    iIntros (T) "[po b]".
+    rewrite storage_bulk_inv_singleton. unfold storage_inv.
+    unfold p_own.
+    iAssert ((own γ (◯ Inved p) ∧
+        (∃ state : P, T ∗ ▷
+               (own γ (● Inved state) ∗ ⌜pinv state⌝ ∗ f (interp P B storage_mixin state))))%I)
+        with "[po b]" as "x".
+    { iSplit. { iFrame. } 
+      iDestruct ("b" with "po") as "[ex t]".
+      iDestruct "ex" as (P0) "[#own lat]".
+      iDestruct (ownIagree γ P0 _ with "[inv own]") as "eq".
+      { iSplitL. { iFrame "own". } iFrame "inv". }
+      iRewrite "eq" in "lat".
+      iDestruct (bi.later_exist with "lat") as (state) "lat".
+      iExists state. iFrame.
+    }
+    rewrite bi.and_exist_l.
+    iDestruct "x" as (state) "x".
+    iMod (apply_timeless with "x") as "x".
+    iDestruct (stuff1 with "x") as "%pinvs".
+    iDestruct (stuff2 with "x") as "%incll".
+    iDestruct "x" as "[_ [t [o [p latf]]]]".
+    
+    unfold storage_protocol_guards in g.
+    unfold "≼" in incll. destruct incll as [z incll].
+    assert (pinv (p ⋅ z)) as pinv_pz.
+        { destruct storage_mixin. destruct protocol_mixin0. setoid_rewrite <- incll. trivial. }
+    have gz := g z pinv_pz.
+    unfold "≼" in gz. destruct gz as [y gz].
+    assert (interp P B storage_mixin state ≡ b ⋅ y) as ieqop.
+    { destruct storage_mixin. unfold interp. 
+        setoid_rewrite incll. trivial. }
+    
+    unfold wf_prop_map in wf.
+    destruct wf as [fprop [funit fop]].
+    
+    assert (✓ (b ⋅ y)) as is_val.
+    { destruct storage_mixin. destruct base_ra_mixin0.
+        setoid_rewrite <- ieqop. apply interp_val0. trivial. }
+        
+    setoid_rewrite ieqop.
+    setoid_rewrite fop; trivial.
+    
+    rewrite bi.later_sep. 
+    iDestruct "latf" as "[fb fy]".
+    iModIntro.
+    iFrame "fb".
+    iIntros "fb".
+    iFrame "t".
+    iExists ((∃ state0 : P,
+              own γ (● Inved state0) ∗ ⌜pinv state0⌝ ∗ f (interp P B storage_mixin state0))%I).
+    iFrame "inv".
+    iNext. iExists state. iFrame.
+    setoid_rewrite ieqop. setoid_rewrite fop; trivial. iFrame.
+    
+    Unshelve.
+    apply inhabits.
+    apply exists_inhabited.
+    apply inhabitant.
+      
       
 
 Print own.
